xorlist proof refactored

clightdm/decompiler/ClightDmgen.v
@@ -1,6 +1,6 @@
 Require Import Coqlib.
 Require Import ITreelib.
-Require Import Skeleton.
+Require Import ClightDmSkel.
 Require Import PCM.
 Require Import STS Behavior.
 Require Import Any.
@@ -17,7 +17,7 @@ Require Import ClightDmExprgen.
 Section HIDE.
 
   Definition hide (p: positive) {A: Type} {a: A} := a.
-  Arguments hide _ {A} {a}: simpl never.  
+  Arguments hide _ {A} {a}: simpl never.
 
 End HIDE.
 
@@ -26,8 +26,8 @@ Section Clight.
 Context {eff : Type -> Type}.
 Context {HasCall : callE -< eff}.
 Context {HasEvent : eventE -< eff}.
-Variable ske: Sk.sem.
-Let skenv: SkEnv.t := Sk.load_skenv ske.
+Variable sk: Sk.t.
+Let skenv: SkEnv.t := load_skenv sk.
 Variable ce: comp_env.
 
 Definition id_list_norepet_c: list ident -> bool :=
@@ -72,38 +72,42 @@ Section DECOMP.
 
   Definition _sassign_c e le a1 a2 :=
     tau;;
-    vp <- eval_lvalue_c ske ce e le a1;;
-    v <- eval_expr_c ske ce e le a2;; 
+    vp <- eval_lvalue_c sk ce e le a1;;
+    v <- eval_expr_c sk ce e le a2;; 
     v' <- sem_cast_c v (typeof a2) (typeof a1);;
     assign_loc_c ce (typeof a1) vp v'.
+
 
   Definition _scall_c e le a al
     : itree eff val :=
     match Cop.classify_fun (typeof a) with
     | Cop.fun_case_f tyargs tyres cconv =>
       tau;;
-      vf <- eval_expr_c ske ce e le a;;
-      vargs <- eval_exprlist_c ske ce e le al tyargs;;
+      vf <- eval_expr_c sk ce e le a;;
+      vargs <- eval_exprlist_c sk ce e le al tyargs;;
       match vf with
       | Vptr b ofs =>
           if Ptrofs.eq_dec ofs Ptrofs.zero
           then
-            '(id, gd) <- (nth_error ske (pred (Pos.to_nat b)))?;;
-            fd <- (match gd with inr (Gfun fd) => Some fd | _ => None end)?;;
-            if type_eq (type_of_clightdm_fundef fd)
-                (Tfunction tyargs tyres cconv)
-            then match fd with
-                 | CInternal _ => ccallU (string_of_ident id) vargs
-                 | CExternal CEF_malloc _ => ccallU "malloc" vargs
-                 | CExternal CEF_free _ => ccallU "free" vargs
-                 (* this is for builtin memcpy, uncallable in standard C *)
-                 (* | External (EF_memcpy al sz) _ _ _ => ccallU "memcpy" (al, sz, vargs) *)
-                 | CExternal CEF_capture _ => ccallU "capture" vargs
-                 | _ => triggerUB
-                 end
+            (* skeleton name = function name *)
+            '(gsym, gd) <- (nth_error sk (pred (Pos.to_nat b)))?;;
+            fd <- (match gd with Gfun fd => Some fd | _ => None end)?;;
+            if type_eq (type_of_fundef fd) (Tfunction tyargs tyres cconv)
+            then 
+              match fd with
+              | Internal _
+              (* malloc, free, capture's name in c level should equal to function name in ccr level *)
+              | External EF_malloc _ _ _
+              | External EF_free _ _ _ 
+              | External EF_capture _ _ _ => ccallU gsym vargs
+              (* this is for builtin memcpy, uncallable in standard C *)
+              (* | EF_memcpy al sz => ccallU "memcpy" (al, sz, vargs) *)
+              (* there's no system call currently *)
+              | External _ _ _ _ => triggerUB
+              end
             else triggerUB
           else triggerUB
-      | _ => triggerUB (* unreachable b*)
+      | _ => triggerUB
       end
     | _ => triggerUB
     end.
@@ -112,7 +116,7 @@ Section DECOMP.
              (e: env) (le: temp_env) (a: expr)
     : itree eff bool :=
     tau;;
-    v1 <- eval_expr_c ske ce e le a;;
+    v1 <- eval_expr_c sk ce e le a;;
     bool_val_c v1 (typeof a).
 
   Definition sloop_iter_body_one
@@ -199,7 +203,7 @@ Section DECOMP.
 
   Definition blocks_of_env (ce: comp_env) (le: env) :=
     List.map (block_of_binding ce) le.
-  
+
   Definition _sreturn_c
              (retty: type)
              (e: env) (le: temp_env)
@@ -209,7 +213,7 @@ Section DECOMP.
     | None => tau;;Ret Vundef
     | Some a =>
       tau;;
-      v <- eval_expr_c ske ce e le a;;
+      v <- eval_expr_c sk ce e le a;;
       sem_cast_c v (typeof a) retty
     end.
 
@@ -227,7 +231,7 @@ Section DECOMP.
       Ret (e, le, None, None)
     | Sset id a =>
       tau;;
-      v <- eval_expr_c ske ce e le a ;;
+      v <- eval_expr_c sk ce e le a ;;
       let le' := alist_add (string_of_ident id) v le in
       Ret (e, le', None, None)
     | Scall optid a al =>
@@ -235,16 +239,16 @@ Section DECOMP.
         Ret (e, (match optid with Some id => alist_add (string_of_ident id) v le | None => le end), None, None)
     | Sbuiltin optid ef tyargs al =>
       tau;;
-      vargs <- eval_exprlist_c ske ce e le al tyargs;;
+      vargs <- eval_exprlist_c sk ce e le al tyargs;;
       match ef with
       | EF_malloc => v <- ccallU "malloc" vargs;;
         Ret (e, (match optid with Some id => alist_add (string_of_ident id) v le | None => le end), None, None)
-      | EF_free => v <- ccallU "free" vargs;;
+      | EF_free => v <- ccallU "mfree" vargs;;
+        Ret (e, (match optid with Some id => alist_add (string_of_ident id) v le | None => le end), None, None)
+      | EF_capture => v <- ccallU "capture" vargs;;
         Ret (e, (match optid with Some id => alist_add (string_of_ident id) v le | None => le end), None, None)
       (* this is for builtin memcpy, uncallable in standard C *)
       (* | EF_memcpy al sz => ccallU "memcpy" (al, sz, vargs) *)
-      | EF_capture => v <- ccallU "capture" vargs;;
-        Ret (e, (match optid with Some id => alist_add (string_of_ident id) v le | None => le end), None, None)
       | _ => triggerUB
       end
     | Ssequence s1 s2 =>
@@ -298,71 +302,6 @@ Section DECOMP.
     end);; v <- v?;;
     Ret v.
 
-  (* Lemma unfold_decomp_stmt :
-    decomp_stmt
-    = fun retty stmt e le =>
-        match stmt with
-        | Sskip =>
-          Ret (e, le, None, None)
-        | Sassign a1 a2 =>
-          _sassign_c e le a1 a2;;;
-          Ret (e, le, None, None)
-        | Sset id a =>
-          tau;;
-          v <- eval_expr_c sk ce e le a ;;
-          let le' := PTree.set id v le in
-          Ret (e, le', None, None)
-        | Scall optid a al =>
-            v <- _scall_c e le a al;;
-            Ret (e, (set_opttemp optid v le), None, None)
-        | Sbuiltin optid ef tyargs al =>
-          tau;;
-          vargs <- eval_exprlist_c sk ce e le al tyargs;;
-          match ef with
-          | EF_malloc => ccallU "malloc" vargs
-          | EF_free => ccallU "free" vargs
-          (* this is for builtin memcpy, uncallable in standard C *)
-          (* | EF_memcpy al sz => ccallU "memcpy" (al, sz, vargs) *)
-          | EF_capture => ccallU "capture" vargs
-          | _ => triggerUB
-          end
-        | Ssequence s1 s2 =>
-          '(e', le', bc, v) <- tau;;decomp_stmt retty s1 e le;;
-                            (* this is for steps *)
-          match v with
-          | Some retval =>
-            Ret (e', le', None, v)
-          | None =>
-            match bc with
-            | None =>
-              tau;;decomp_stmt retty s2 e' le'
-            | Some true =>
-              tau;;Ret (e', le', bc, None)
-            | Some false =>
-              tau;;Ret (e', le', bc, None)
-            end
-          end
-        | Sifthenelse a s1 s2 =>
-          b <- _site_c e le a;;
-          if (b: bool) then (decomp_stmt retty s1 e le)
-          else (decomp_stmt retty s2 e le)
-        | Sloop s1 s2 =>
-          let itr1 := decomp_stmt retty s1 in
-          let itr2 := decomp_stmt retty s2 in
-          _sloop_itree e le itr1 itr2
-        | Sbreak =>
-          Ret (e, le, Some true, None)
-        | Scontinue =>
-          Ret (e, le, Some false, None)
-        | Sreturn oa =>
-          v <- _sreturn_c retty e le oa;;
-          Ret (e, le, None, Some v)
-        | _ =>
-          (* not supported *)
-          triggerUB
-        end.
-    Proof. repeat (apply func_ext; i). destruct x0; et. Qed. *)
-  
 End DECOMP.
 End Clight.
 (* Notation call_data := (block * (* fundef * *) list val * mem)%type. *)
@@ -566,7 +505,6 @@ Section DECOMP_PROG.
   Definition get_ce (prog: Clight.program) : comp_env :=
     List.map (fun '(id, p) => (string_of_ident id, p)) (PTree.elements prog.(prog_comp_env)).
 
-  (* Context `{SystemEnv}. *)
   Variable prog: Clight.program.
   Let ce: comp_env := get_ce prog.
   Let defs: list (ident * globdef Clight.fundef type) := prog.(prog_defs).
@@ -576,81 +514,41 @@ Section DECOMP_PROG.
   (* Fixpoint get_source_name (filename : string) := *)
   (*   String.substring 0 (String.length filename - 2) filename. *)
 
-  Fixpoint decomp_fundefs (ske: Sk.sem)
-           (defs: list (ident * globdef Clight.fundef type))
-    : list (ident * (list val -> itree Es val)) :=
+  Fixpoint decomp_fundefs (sk: Sk.t) (defs: list (ident * globdef Clight.fundef type)) :=
     match defs with
     | [] => []
     | (id, gdef) :: defs' =>
       match gdef with
-      | Gvar _ => decomp_fundefs ske defs'
+      | Gvar _ => decomp_fundefs sk defs'
       | Gfun fd =>
         match fd with
         | Internal f => 
-          (id, fun vl => 
-                  v <- decomp_func ske ce f vl;; 
-                  (if Pos.eq_dec id (ident_of_string "main")
-                   then (match v with Vint _ => Ret v | _ => triggerUB end)
-                   else Ret v)) :: decomp_fundefs ske defs'
-        | _ => decomp_fundefs ske defs'
+          (string_of_ident id,
+            cfunU (E:=Es) (fun vl =>
+                            if Pos.eq_dec id prog.(prog_main)
+                            then if type_eq (type_of_function f) (Tfunction Tnil type_int32s cc_default)
+                                  then v <- decomp_func sk ce f vl;; 
+                                      match v with
+                                      | Vint _ => Ret v
+                                      | _ => triggerUB
+                                      end
+                                  else triggerUB
+                            else decomp_func sk ce f vl)) :: decomp_fundefs sk defs'
+        | _ => decomp_fundefs sk defs'
         end
       end
     end.
-  
-  Definition ef2cef (ef: external_function) : extfun :=
-    match ef with
-    | EF_external _ _ => CEF_external
-    | EF_builtin name sg => CEF_builtin name sg 
-    | EF_runtime name sg => CEF_runtime name sg
-    | EF_vload chunk => CEF_vload chunk
-    | EF_vstore chunk => CEF_vstore chunk
-    | EF_malloc => CEF_malloc 
-    | EF_free => CEF_free 
-    | EF_memcpy sz al => CEF_memcpy sz al
-    | EF_annot id str typl => CEF_annot id str typl
-    | EF_annot_val id str typ => CEF_annot_val id str typ
-    | EF_inline_asm str sg strs => CEF_inline_asm str sg strs
-    | EF_debug pos id typl => CEF_debug pos id typl
-    | EF_capture => CEF_capture
+
+  Fixpoint get_sk (defs: list (ident * globdef Clight.fundef type)) : Sk.t :=
+    match defs with
+    | [] => []
+    | (id, Gvar gv) :: defs' => (string_of_ident id, Gvar gv) :: get_sk defs'
+    | (id, Gfun (Internal f)) :: defs' => (string_of_ident id, Gfun (Internal f)) :: get_sk defs'
+    | _ :: defs' => get_sk defs'
     end.
 
-  Fixpoint get_sk_aux
-    (defs: list (ident * globdef Clight.fundef type)) (p: PTree.t clightdm_globaldata) 
-      : Sk.t :=
-    match defs with
-    | [] => p
-    | (id, gdef) :: defs' => 
-      match gdef with
-           | Gvar gv => 
-              PTree.set id
-                (inr (Gvar (F:=clightdm_fundef) gv))
-                (get_sk_aux defs' p)
-           | Gfun fd =>
-              match fd with
-              | Internal f =>
-                PTree.set id
-                  (inr (Gfun (CInternal (type_of_fundef fd))))
-                  (get_sk_aux defs' p)
-              | External (EF_external name sg) tyl rty cc =>
-                if dec id (ident_of_string name) && signature_eq sg (signature_of_type tyl rty cc)
-                then PTree.set id
-                      (inr (Gfun (CExternal CEF_external (type_of_fundef fd))))
-                      (get_sk_aux defs' p)
-                else PTree.set id (inl true) (get_sk_aux defs' p)
-              | External ef _ _ _ =>
-                PTree.set id
-                  (inr (Gfun (CExternal (ef2cef ef) (type_of_fundef fd))))
-                  (get_sk_aux defs' p)
-              end
-            end
-    end
-  .
-
-  Definition get_sk (defs: list (ident * globdef Clight.fundef type)) : Sk.t :=
-    get_sk_aux defs (PTree.empty _).
-
-  Definition modsem (ske: Sk.sem) : ModSem.t := {|
-    ModSem.fnsems := List.map (fun '(fn, f) => (string_of_ident fn, cfunU f)) (decomp_fundefs ske defs);
+  Definition modsem (sk: Sk.t) : ModSem.t := {|
+    ModSem.fnsems := decomp_fundefs sk defs;
     ModSem.mn := mn;
     ModSem.initial_st := tt↑;
   |}.
