clight_examples/xorlist/xorlist01proof.v
@@ -3,15 +3,14 @@ Require Import Any.
 Require Import STS.
 Require Import Behavior.
 Require Import ModSem.
-Require Import Skeleton.
 Require Import SimModSem.
 Require Import PCM.
 Require Import HoareDef.
 Require Import STB.
 Require Import HTactics ProofMode.
 Require Import HSim IProofMode.
-Require Import ClightDmExprgen ClightDmgen.
-Require Import ClightDmMem1.
+Require Import ClightDmSkel ClightDmExprgen ClightDmgen.
+Require Import ClightDmMem0 ClightDmMem1.
 Require Import CIProofMode.
 Require Import xorlist.
 Require Import xorlist0.
@@ -66,7 +65,7 @@ Section PROOF.
   Context `{@GRA.inG blocksizeRA Σ}.
   Context `{@GRA.inG blockaddressRA Σ}.
   
-  Variable GlobalStb : Sk.sem -> gname -> option fspec.
+  Variable GlobalStb : Sk.t -> gname -> option fspec.
   Hypothesis STBINCL : forall sk, stb_incl (to_stb xorStb) (GlobalStb sk).
   Hypothesis MEMINCL : forall sk, stb_incl (to_stb MemStb) (GlobalStb sk).
 
@@ -82,13 +81,14 @@ Section PROOF.
 
   Section SIMFUNS.
   Variable sk: Sk.t.
-  Hypothesis SKINCL : Sk.extends (xorlist0.xor.(Mod.sk)) sk.
-  Hypothesis SKWF : Sk.wf (Sk.canon sk).
+  Hypothesis SKINCL1 : Sk.le (xorlist0.xor.(Mod.sk)) sk.
+  Hypothesis SKINCL2 : Sk.le (ClightDmMem0.Mem.(Mod.sk)) sk.
+  Hypothesis SKWF : Sk.wf sk.
 
   Lemma sim_add_tl :
     sim_fnsem wf top2
-      ("add_tl", fun_to_tgt "xorlist" (GlobalStb (Sk.canon sk)) (mk_pure add_tl_spec))
-      ("add_tl", cfunU (decomp_func (Sk.canon sk) ce f_add_tl)).
+      ("add_tl", fun_to_tgt "xorlist" (GlobalStb sk) (mk_pure add_tl_spec))
+      ("add_tl", cfunU (decomp_func sk ce f_add_tl)).
   Proof.
     Opaque encode_val.
     Opaque cast_to_ptr.
@@ -99,10 +99,13 @@ Section PROOF.
     destruct (build_composite_env'). ss.
     get_composite ce e.
 
-    dup SKINCL. rename SKINCL0 into SKINCLENV.
-    apply Sk.incl_incl_env in SKINCLENV.
-    unfold Sk.incl_env in SKINCLENV.
-    pose proof Sk.sk_incl_gd as SKINCLGD.
+    dup SKINCL1. rename SKINCL0 into SKINCLENV1.
+    apply incl_incl_env in SKINCLENV1.
+    unfold incl_env in SKINCLENV1.
+    dup SKINCL2. rename SKINCL0 into SKINCLENV2.
+    apply incl_incl_env in SKINCLENV2.
+    unfold incl_env in SKINCLENV2.
+    pose proof sk_incl_gd as SKINCLGD.
 
     apply isim_fun_to_tgt; auto.
     unfold f_add_hd. i; ss.
@@ -118,8 +121,8 @@ Section PROOF.
     (* node* entry = (node* ) malloc(sizeof(node)) start *)
     unhide. hred_r. unhide. remove_tau. unhide. remove_tau.
 
-    hexploit SKINCLENV.
-    { instantiate (2:="malloc"). ss. }
+    hexploit SKINCLENV2.
+    { instantiate (2:="malloc"). et. }
     i. des. ss. rewrite FIND. rename FIND into malloc_loc.
     hred_r. des_ifs_safe.
     rewrite cast_ptrofs.
@@ -127,7 +130,7 @@ Section PROOF.
     clear Heq e. hred_r.
 
     replace (pred _) with blk by nia.
-    erewrite SKINCLGD; et.
+    erewrite SKINCLGD; et; [|ss; et].
     hred_r. ss.
     iApply isim_apc. iExists (Some (20%nat : Ord.t)).
     rewrite co_co_sizeof.
@@ -136,7 +139,7 @@ Section PROOF.
     iSplitL "INV"; iFrame.
     { iPureIntro. ss. }
     iIntros (st_src0 st_tgt0 p_new m_new) "[INV [[% new_point] new_ofs]]".
-    set (Z.to_nat _) as si. vm_compute in si. unfold si. clear si.
+    change (Z.to_nat _) with 16.
     rename H3 into m_new_size.
 
     hred_r. unhide. remove_tau. 
@@ -376,11 +379,13 @@ Section PROOF.
     iExists _,_,_,_,_,_,_,_. iFrame. iSplit; ss.
     rewrite <- (rev_involutive ((rev lfull ++ _) ++ _)).
     iApply rev_xorlist. rewrite rev_app_distr.
-    vm_compute (rev [_]). ss. rewrite rev_app_distr.
-    vm_compute (rev [_]). ss.
+    change (rev [Vlong item]) with [Vlong item].
+    ss. rewrite rev_app_distr.
+    change (rev [Vlong i]) with [Vlong i].
+    ss.
     iExists _,_,_. iFrame. rewrite Ptrofs.xor_zero_l. iFrame. iSplit; ss.
     rewrite <- Heq0.
-    
+
     iPoseProof (equiv_dup with "tl_addr") as "[tl_addr tl_addr']".
     iCombine "tl_addr' tl_point" as "tl_point".
     iPoseProof (equiv_point_comm with "tl_point") as "tl_point".
@@ -399,8 +404,8 @@ Section PROOF.
 
   Lemma sim_add_hd :
     sim_fnsem wf top2
-      ("add_hd", fun_to_tgt "xorlist" (GlobalStb (Sk.canon sk)) (mk_pure add_hd_spec))
-      ("add_hd", cfunU (decomp_func (Sk.canon sk) ce f_add_hd)).
+      ("add_hd", fun_to_tgt "xorlist" (GlobalStb sk) (mk_pure add_hd_spec))
+      ("add_hd", cfunU (decomp_func sk ce f_add_hd)).
   Proof.
     Opaque encode_val.
     Opaque cast_to_ptr.
@@ -411,10 +416,13 @@ Section PROOF.
     destruct (build_composite_env'). ss.
     get_composite ce e.
 
-    dup SKINCL. rename SKINCL0 into SKINCLENV.
-    apply Sk.incl_incl_env in SKINCLENV.
-    unfold Sk.incl_env in SKINCLENV.
-    pose proof Sk.sk_incl_gd as SKINCLGD.
+    dup SKINCL1. rename SKINCL0 into SKINCLENV1.
+    apply incl_incl_env in SKINCLENV1.
+    unfold incl_env in SKINCLENV1.
+    dup SKINCL2. rename SKINCL0 into SKINCLENV2.
+    apply incl_incl_env in SKINCLENV2.
+    unfold incl_env in SKINCLENV2.
+    pose proof sk_incl_gd as SKINCLGD.
 
     apply isim_fun_to_tgt; auto.
     unfold f_add_hd. i; ss.
@@ -430,8 +438,8 @@ Section PROOF.
     (* node* entry = (node* ) malloc(sizeof(node)) start *)
     unhide. hred_r. unhide. remove_tau. unhide. remove_tau.
 
-    hexploit SKINCLENV.
-    { instantiate (2:="malloc"). ss. }
+    hexploit SKINCLENV2.
+    { instantiate (2:="malloc"). et. }
     i. des. ss. rewrite FIND. rename FIND into malloc_loc.
     hred_r. des_ifs_safe.
     rewrite cast_ptrofs.
@@ -439,7 +447,7 @@ Section PROOF.
     clear Heq e. hred_r.
 
     replace (pred _) with blk by nia.
-    erewrite SKINCLGD; et.
+    erewrite SKINCLGD; et; [|ss; et].
     hred_r. ss.
     iApply isim_apc. iExists (Some (20%nat : Ord.t)).
     rewrite co_co_sizeof.
@@ -448,7 +456,7 @@ Section PROOF.
     iSplitL "INV"; iFrame.
     { iPureIntro. ss. }
     iIntros (st_src0 st_tgt0 p_new m_new) "[INV [[% new_point] new_ofs]]".
-    set (Z.to_nat _) as si. vm_compute in si. unfold si. clear si.
+    change (Z.to_nat _) with 16.
     rename H3 into m_new_size.
 
     hred_r. unhide. remove_tau. 
@@ -684,7 +692,7 @@ Section PROOF.
     iExists _,_,_,_,_,_,_,_. iFrame. iSplit; ss.
     iExists _,_,_. iFrame. rewrite Ptrofs.xor_zero_l. iFrame. iSplit; ss.
     rewrite <- Heq0.
-    
+
     iPoseProof (equiv_dup with "hd_addr") as "[hd_addr hd_addr']".
     iCombine "hd_addr' hd_point" as "hd_point".
     iPoseProof (equiv_point_comm with "hd_point") as "hd_point".
@@ -703,8 +711,8 @@ Section PROOF.
 
   Lemma sim_delete_tl :
     sim_fnsem wf top2
-      ("delete_tl", fun_to_tgt "xorlist" (GlobalStb (Sk.canon sk)) (mk_pure delete_tl_spec))
-      ("delete_tl", cfunU (decomp_func (Sk.canon sk) ce f_delete_tl)).
+      ("delete_tl", fun_to_tgt "xorlist" (GlobalStb sk) (mk_pure delete_tl_spec))
+      ("delete_tl", cfunU (decomp_func sk ce f_delete_tl)).
   Proof.
     Opaque encode_val.
     econs; ss. red.
@@ -714,10 +722,13 @@ Section PROOF.
     destruct (build_composite_env'). ss.
     get_composite ce e.
 
-    dup SKINCL. rename SKINCL0 into SKINCLENV.
-    apply Sk.incl_incl_env in SKINCLENV.
-    unfold Sk.incl_env in SKINCLENV.
-    pose proof Sk.sk_incl_gd as SKINCLGD.
+    dup SKINCL1. rename SKINCL0 into SKINCLENV1.
+    apply incl_incl_env in SKINCLENV1.
+    unfold incl_env in SKINCLENV1.
+    dup SKINCL2. rename SKINCL0 into SKINCLENV2.
+    apply incl_incl_env in SKINCLENV2.
+    unfold incl_env in SKINCLENV2.
+    pose proof sk_incl_gd as SKINCLGD.
 
     apply isim_fun_to_tgt; auto.
     unfold f_delete_hd. i; ss.
@@ -788,7 +799,7 @@ Section PROOF.
     iPoseProof (decode_encode_ptr_ofs with "tl_ofs") as "%". rewrite H3. rename H3 into tl_old_deen.
     iApply isim_ccallU_cmp_ptr4; ss; oauto.
     iSplitL "INV tl_ofs"; iFrame.
-    { iPureIntro. red. rewrite m_tl_size. vm_compute (size_chunk Mptr). vm_compute (Ptrofs.unsigned Ptrofs.zero). nia. }
+    { iPureIntro. red. rewrite m_tl_size. change (size_chunk Mptr) with 8%Z. change (Ptrofs.unsigned Ptrofs.zero) with 0%Z. nia. }
     iIntros (st_src1 st_tgt1) "[INV tl_ofs]".
     hred_r. destruct (Int.eq) eqn: ?; ss; clarify. clear Heqb.
     (* if (hd_old != NULL) end *)
@@ -853,7 +864,7 @@ Section PROOF.
       (* tlH* = NULL start *)
       iPoseProof (points_to_is_ptr with "hd_hdl_point") as "%". rewrite H3. rename H3 into hd_hdl_ptr.
       hred_r. change Archi.ptr64 with true. hred_r.
-      change Archi.ptr64 with true. hred_r.
+      rewrite cast_long; et. hred_r.
 
       iApply isim_ccallU_store; ss; oauto.
       iSplitL "INV hd_hdl_point hd_hdl_ofs"; iFrame.
@@ -864,15 +875,15 @@ Section PROOF.
       hred_r. unhide. remove_tau.
 
       (* free(hd_old) start *)
-      hexploit SKINCLENV.
-      { instantiate (2:="free"). ss. }
+      hexploit SKINCLENV2.
+      { instantiate (2:="free"). et. }
       i. des. ss. rewrite FIND. rename FIND into free_loc. hred_r.
 
       iPoseProof ((@point_cast_ptr _ _ _ _ Es) with "tl_point_item") as "%".
       rewrite H3. rename H3 into tl_old_cast. hred_r. des_ifs_safe. clear e.
 
       replace (pred _) with blk by nia.
-      erewrite SKINCLGD; et. hred_r.
+      erewrite SKINCLGD; et; [|ss; et]. hred_r.
 
       iCombine "tl_point_item tl_point_key" as "tl_point".
       replace (Val.addl tl_old (Vlong _)) 
@@ -886,7 +897,9 @@ Section PROOF.
       iIntros (st_src7 st_tgt7) "INV".
       (* free(hd_old) end *)
 
-      hred_r. unhide. remove_tau. change Archi.ptr64 with true. hred_r.
+      hred_r. unhide. remove_tau. change Archi.ptr64 with true. ss.
+      rewrite cast_long; et. hred_r.
+
 
       (* prove post condition *)
       hred_l. iApply isim_choose_src. iExists _.
@@ -898,7 +911,7 @@ Section PROOF.
 
       iApply isim_ccallU_cmp_ptr3; ss; oauto.
       iSplitL "INV tl_prev_ofs"; iFrame.
-      { iPureIntro. red. rewrite m_tl_prev_size. vm_compute (Ptrofs.unsigned Ptrofs.zero). vm_compute (size_chunk Mptr). nia. }
+      { iPureIntro. red. rewrite m_tl_prev_size. change (Ptrofs.unsigned Ptrofs.zero) with 0%Z. change (size_chunk Mptr) with 8%Z. nia. }
       iIntros (st_src5 st_tgt5) "[INV tl_prev_ofs]".
       (* if (hd_new == NULL) end *)
           
@@ -937,8 +950,8 @@ Section PROOF.
       rewrite get_co. hred_r. rewrite co_co_members.
       ss. change Archi.ptr64 with true. hred_r. 
       do 2 rewrite ptrofs_cast_ptr. hred_r. des_ifs_safe.
-      hred_r. change Archi.ptr64 with true. hred_r. 
-      
+      hred_r. rewrite cast_long; et. hred_r.
+
       change (Vptrofs (Ptrofs.repr (Coqlib.align _ _))) with (Vptrofs (Ptrofs.repr 8)).
       iApply isim_ccallU_store; ss; oauto.
       iSplitL "INV tl_prev_point_key tl_prev_ofs"; iFrame.
@@ -949,13 +962,13 @@ Section PROOF.
       hred_r. unhide. remove_tau.
 
       (* free(hd_old) start *)
-      hexploit SKINCLENV.
-      { instantiate (2:="free"). ss. }
+      hexploit SKINCLENV2.
+      { instantiate (2:="free"). et. }
       i. des. ss. rewrite FIND. rename FIND into free_loc. hred_r. 
       rewrite tl_old_cast. hred_r.
       destruct (Ptrofs.eq_dec) eqn:?; clarify. clear e Heqs.
       replace (pred _) with blk by nia.
-      erewrite SKINCLGD; et. hred_r.
+      erewrite SKINCLGD; et; [|ss; et]. hred_r.
 
       iCombine "tl_point_item tl_point_key" as "tl_point".
       iPoseProof (points_to_collect with "tl_point") as "tl_point".
@@ -966,7 +979,8 @@ Section PROOF.
       iIntros (st_src12 st_tgt12) "INV".
       (* free(hd_old) end *)
 
-      hred_r. unhide. remove_tau. change Archi.ptr64 with true. hred_r.
+      hred_r. unhide. remove_tau. change Archi.ptr64 with true. ss.
+      rewrite cast_long; et. hred_r.
 
       (* prove post condition *)
       hred_l. iApply isim_choose_src. iExists _.
@@ -976,7 +990,7 @@ Section PROOF.
       iExists _,_,_,_,_,_,_,_. iFrame. iSplit; ss.
       rewrite removelast_last. rewrite <- (rev_involutive (rev lnext ++ _)).
       iApply rev_xorlist. rewrite rev_app_distr. rewrite rev_involutive.
-      vm_compute (rev [Vlong tl_prev_item]). ss.
+      change (rev [Vlong tl_prev_item]) with [Vlong tl_prev_item]. ss.
       iExists _,_,_. iFrame. rewrite Ptrofs.xor_zero_l.
       iSplit; ss. replace (Vlong (Int64.xor i i0)) with (Vptrofs i_tl_pp); et.
       clear - Heq Heq0. unfold Vptrofs in *. des_ifs. f_equal.
@@ -989,8 +1003,8 @@ Section PROOF.
 
   Lemma sim_delete_hd :
     sim_fnsem wf top2
-      ("delete_hd", fun_to_tgt "xorlist" (GlobalStb (Sk.canon sk)) (mk_pure delete_hd_spec))
-      ("delete_hd", cfunU (decomp_func (Sk.canon sk) ce f_delete_hd)).
+      ("delete_hd", fun_to_tgt "xorlist" (GlobalStb sk) (mk_pure delete_hd_spec))
+      ("delete_hd", cfunU (decomp_func sk ce f_delete_hd)).
   Proof.
     Opaque encode_val.
     econs; ss. red.
@@ -1000,10 +1014,13 @@ Section PROOF.
     destruct (build_composite_env'). ss.
     get_composite ce e.
 
-    dup SKINCL. rename SKINCL0 into SKINCLENV.
-    apply Sk.incl_incl_env in SKINCLENV.
-    unfold Sk.incl_env in SKINCLENV.
-    pose proof Sk.sk_incl_gd as SKINCLGD.
+    dup SKINCL1. rename SKINCL0 into SKINCLENV1.
+    apply incl_incl_env in SKINCLENV1.
+    unfold incl_env in SKINCLENV1.
+    dup SKINCL2. rename SKINCL0 into SKINCLENV2.
+    apply incl_incl_env in SKINCLENV2.
+    unfold incl_env in SKINCLENV2.
+    pose proof sk_incl_gd as SKINCLGD.
 
     apply isim_fun_to_tgt; auto.
     unfold f_delete_hd. i; ss.
@@ -1070,7 +1087,7 @@ Section PROOF.
     iPoseProof (decode_encode_ptr_ofs with "hd_ofs") as "%". rewrite H3. rename H3 into hd_old_deen.
     iApply isim_ccallU_cmp_ptr4; ss; oauto.
     iSplitL "INV hd_ofs"; iFrame.
-    { iPureIntro. red. rewrite m_hd_size. vm_compute (size_chunk Mptr). vm_compute (Ptrofs.unsigned Ptrofs.zero). nia. }
+    { iPureIntro. red. rewrite m_hd_size. change (size_chunk Mptr) with 8%Z. change (Ptrofs.unsigned Ptrofs.zero) with 0%Z. nia. }
     iIntros (st_src1 st_tgt1) "[INV hd_ofs]".
     hred_r. destruct (Int.eq) eqn: ?; ss; clarify. clear Heqb.
     (* if (hd_old != NULL) end *)
@@ -1135,7 +1152,7 @@ Section PROOF.
       (* tlH* = NULL start *)
       iPoseProof (points_to_is_ptr with "tl_hdl_point") as "%". rewrite H3. rename H3 into tl_hdl_ptr.
       hred_r. change Archi.ptr64 with true. hred_r.
-      change Archi.ptr64 with true. hred_r.
+      rewrite cast_long; et. hred_r.
 
       iApply isim_ccallU_store; ss; oauto.
       iSplitL "INV tl_hdl_point tl_hdl_ofs"; iFrame.
@@ -1146,15 +1163,15 @@ Section PROOF.
       hred_r. unhide. remove_tau.
 
       (* free(hd_old) start *)
-      hexploit SKINCLENV.
-      { instantiate (2:="free"). ss. }
+      hexploit SKINCLENV2.
+      { instantiate (2:="free"). et. }
       i. des. ss. rewrite FIND. rename FIND into free_loc. hred_r.
 
       iPoseProof ((@point_cast_ptr _ _ _ _ Es) with "hd_point_item") as "%".
       rewrite H3. rename H3 into hd_old_cast. hred_r. des_ifs_safe. clear e.
 
       replace (pred _) with blk by nia.
-      erewrite SKINCLGD; et. hred_r.
+      erewrite SKINCLGD; et; [|ss; et]. hred_r.
 
       iCombine "hd_point_item hd_point_key" as "hd_point".
       replace (Val.addl tl_old (Vlong _)) 
@@ -1168,7 +1185,8 @@ Section PROOF.
       iIntros (st_src7 st_tgt7) "INV".
       (* free(hd_old) end *)
 
-      hred_r. unhide. remove_tau. change Archi.ptr64 with true. hred_r.
+      hred_r. unhide. remove_tau. change Archi.ptr64 with true. ss.
+      rewrite cast_long; et. hred_r.
 
       (* prove post condition *)
       hred_l. iApply isim_choose_src. iExists _.
@@ -1180,7 +1198,7 @@ Section PROOF.
 
       iApply isim_ccallU_cmp_ptr3; ss; oauto.
       iSplitL "INV hd_next_ofs"; iFrame.
-      { iPureIntro. red. rewrite m_hd_next_size. vm_compute (Ptrofs.unsigned Ptrofs.zero). vm_compute (size_chunk Mptr). nia. }
+      { iPureIntro. red. rewrite m_hd_next_size. change (Ptrofs.unsigned Ptrofs.zero) with 0%Z. change (size_chunk Mptr) with 8%Z. nia. }
       iIntros (st_src5 st_tgt5) "[INV hd_next_ofs]".
       (* if (hd_new == NULL) end *)
           
@@ -1219,8 +1237,8 @@ Section PROOF.
       rewrite get_co. hred_r. rewrite co_co_members.
       ss. change Archi.ptr64 with true. hred_r. 
       do 2 rewrite ptrofs_cast_ptr. hred_r. des_ifs_safe.
-      hred_r. change Archi.ptr64 with true. hred_r. 
-      
+      hred_r. rewrite cast_long; et. hred_r.
+
       change (Vptrofs (Ptrofs.repr (Coqlib.align _ _))) with (Vptrofs (Ptrofs.repr 8)).
       iApply isim_ccallU_store; ss; oauto.
       iSplitL "INV hd_next_point_key hd_next_ofs"; iFrame.
@@ -1231,13 +1249,13 @@ Section PROOF.
       hred_r. unhide. remove_tau.
 
       (* free(hd_old) start *)
-      hexploit SKINCLENV.
-      { instantiate (2:="free"). ss. }
+      hexploit SKINCLENV2.
+      { instantiate (2:="free"). et. }
       i. des. ss. rewrite FIND. rename FIND into free_loc. hred_r. 
       rewrite hd_old_cast. hred_r.
       destruct (Ptrofs.eq_dec) eqn:?; clarify. clear e Heqs.
       replace (pred _) with blk by nia.
-      erewrite SKINCLGD; et. hred_r.
+      erewrite SKINCLGD; et; [|ss; et]. hred_r.
 
       iCombine "hd_point_item hd_point_key" as "hd_point".
       iPoseProof (points_to_collect with "hd_point") as "hd_point".
@@ -1248,7 +1266,7 @@ Section PROOF.
       iIntros (st_src12 st_tgt12) "INV".
       (* free(hd_old) end *)
 
-      hred_r. unhide. remove_tau. change Archi.ptr64 with true. hred_r.
+      hred_r. unhide. remove_tau. change Archi.ptr64 with true. ss. rewrite cast_long; et. hred_r.
 
       (* prove post condition *)
       hred_l. iApply isim_choose_src. iExists _.
@@ -1265,179 +1283,19 @@ Section PROOF.
       rewrite Ptrofs.xor_idem.
       rewrite Ptrofs.xor_zero_l. et.
   Qed.
-  (* Lemma sim_encrypt :
-    sim_fnsem wf top2
-      ("encrypt", fun_to_tgt "xorlist" (GlobalStb (Sk.canon sk)) (mk_pure encrypt_spec))
-      ("encrypt", cfunU (decomp_func (Sk.canon sk) ce f_encrypt)).
-  Proof.
-    (* econs; ss. red.
-
-    unfold prog in ce. unfold mkprogram in ce.
-    destruct (build_composite_env').
-    get_composite ce e.
-
-    apply isim_fun_to_tgt; auto. i; ss.
-    unfold decomp_func, function_entry_c. ss.
-    init_hide.
-
-    iIntros "[INV PRE]".
-    destruct x as [?|[?|?]]; ss.
-    - unfold encrypt_hoare1 in *. des_ifs. ss.
-      iDestruct "PRE" as "[[[% ALIVE0] ALIVE1] %]".
-      clarify. hred_r. unhide. remove_tau. unhide. remove_tau. 
-      iPoseProof (liveness_ptr with "ALIVE0") as "%".
-      unfold cast_to_ptr in H3. rewrite H3. hred_r.
-
-      iApply isim_apc. iExists (Some (2%nat : Ord.t)).
-      iApply isim_ccallU_capture2; ss; oauto.
-      iSplitL "INV ALIVE0"; iFrame.
-      iIntros (st_src0 st_tgt0 i) "[INV [ALIVE0 CAP0]]".
-
-      hred_r. remove_tau. unhide. remove_tau. unhide. remove_tau.
-      iPoseProof (liveness_ptr with "ALIVE1") as "%".
-      unfold cast_to_ptr in H4. rewrite H4. hred_r.
-
-      iApply isim_ccallU_capture2; ss; oauto.
-      iSplitL "INV ALIVE1"; iFrame.
-      iIntros (st_src1 st_tgt1 i0) "[INV [ALIVE1 CAP1]]".
-
-      hred_r. remove_tau. unhide. remove_tau. des_ifs_safe.
-      hred_r. hred_l. iApply isim_choose_src. iExists _.
-      iApply isim_ret. iSplits; ss.
-      iFrame. iPureIntro. f_equal.
-      autounfold with ptrArith in *. des_ifs_safe. f_equal.
-      autorewrite with ptrArith; auto with ptrArith.
-      apply lxor_size; auto with ptrArith.
-
-    - unfold encrypt_hoare2 in *. des_ifs. ss.
-      iDestruct "PRE" as "[[% ALIVE] %]".
-      clarify. hred_r. unhide. remove_tau. unhide. remove_tau. 
-      iPoseProof (liveness_ptr with "ALIVE") as "%".
-      unfold cast_to_ptr in H3. rewrite H3. hred_r.
-
-      iApply isim_apc. iExists (Some (2%nat : Ord.t)).
-      iApply isim_ccallU_capture2; ss; oauto.
-      iSplitL "INV ALIVE"; iFrame.
-      iIntros (st_src0 st_tgt0 i) "[INV [ALIVE CAP]]".
-
-      hred_r. remove_tau. unhide. remove_tau. unhide. remove_tau.
-      des_ifs_safe. hred_r. rewrite <- Heq.
-
-      iApply isim_ccallU_capture1; ss; oauto.
-      iSplitL "INV"; iFrame.
-      iIntros (st_src1 st_tgt1) "INV".
-
-      hred_r. remove_tau. unhide. remove_tau. des_ifs_safe.
-      hred_r. hred_l. iApply isim_choose_src. iExists _.
-      iApply isim_ret. iSplits; ss.
-      iFrame. iPureIntro. f_equal. unfold Vnullptr in Heq1.
-      autounfold with ptrArith in *. des_ifs_safe. f_equal.
-      autorewrite with ptrArith; auto with ptrArith.
-      unfold Int64.zero.
-      rewrite Int64.unsigned_repr.
-      2:{ set Int64.max_unsigned. vm_compute in z0. nia. }
-      rewrite Z.lxor_0_r. et.
-
-    - unfold encrypt_hoare3 in *. des_ifs. ss.
-      iDestruct "PRE" as "[[% ALIVE] %]".
-      clarify. hred_r. unhide. remove_tau. unhide. remove_tau. 
-      des_ifs. hred_r. rewrite <- Heq.
-
-      iApply isim_apc. iExists (Some (2%nat : Ord.t)).
-      iApply isim_ccallU_capture1; ss; oauto.
-      iSplitL "INV"; iFrame.
-      iIntros (st_src1 st_tgt1) "INV".
-
-      hred_r. remove_tau. unhide. remove_tau. unhide. remove_tau.
-      iPoseProof (liveness_ptr with "ALIVE") as "%".
-      unfold cast_to_ptr in H3. des_ifs_safe. rewrite H3. hred_r.
-
-      iApply isim_ccallU_capture2; ss; oauto.
-      iSplitL "INV ALIVE"; iFrame.
-      iIntros (st_src0 st_tgt0 i0) "[INV [ALIVE CAP]]".
-
-      hred_r. remove_tau. unhide. remove_tau. des_ifs_safe.
-      hred_r. hred_l. iApply isim_choose_src. iExists _.
-      iApply isim_ret. iSplits; ss.
-      iFrame. iPureIntro. f_equal. unfold Vnullptr in Heq2.
-      autounfold with ptrArith in *. des_ifs_safe.
-  Qed. *)
-  Admitted.
-
-
-  Lemma sim_decrypt :
-    sim_fnsem wf top2
-      ("decrypt", fun_to_tgt "xorlist" (GlobalStb (Sk.canon sk)) (mk_pure decrypt_spec))
-      ("decrypt", cfunU (decomp_func (Sk.canon sk) ce f_decrypt)).
-  Proof.
-    (* econs; ss. red.
-
-    unfold prog in ce. unfold mkprogram in ce.
-    destruct (build_composite_env').
-    get_composite ce e.
-
-    apply isim_fun_to_tgt; auto. i; ss.
-    unfold decomp_func, function_entry_c. ss.
-    init_hide.
-
-    iIntros "[INV PRE]".
-    destruct x as [?|?]; ss.
-    - unfold decrypt_hoare1 in *. des_ifs_safe. ss.
-      iDestruct "PRE" as "[PRE %]".
-      iDestruct "PRE" as (key) "[% ALIVE]". des. clarify.
-      hred_r. unhide. remove_tau. unhide. remove_tau.
-      iPoseProof (liveness_ptr with "ALIVE") as "%".
-      unfold cast_to_ptr in H3. rewrite H3. hred_r.
-
-      iApply isim_apc. iExists (Some (1%nat : Ord.t)).
-      iApply isim_ccallU_capture2; ss; oauto.
-      iSplitL "INV ALIVE"; iFrame.
-      iIntros (st_src0 st_tgt0 i0) "[INV [ALIVE CAP]]".
-
-      hred_r. remove_tau. unhide. remove_tau. des_ifs_safe.
-      hred_r. hred_l. iApply isim_choose_src. iExists _.
-      iApply isim_ret.
-      iFrame. iSplit; ss. iExists _. iFrame.
-      iPureIntro. f_equal.
-      autounfold with ptrArith in *. des_ifs_safe.
-      f_equal. unfold Ptrofs.xor.
-      autorewrite with ptrArith; auto with ptrArith.
-      apply lxor_size; auto with ptrArith.
-
-    - iDestruct "PRE" as "[PRE %]".
-      iDestruct "PRE" as (key) "%". des. clarify.
-      hred_r. unhide. remove_tau. unhide. remove_tau.
-      des_ifs. hred_r. rewrite <- Heq.
-
-      iApply isim_apc. iExists (Some (1%nat : Ord.t)).
-      iApply isim_ccallU_capture1; ss; oauto.
-      iSplitL "INV"; iFrame.
-      iIntros (st_src0 st_tgt0) "INV".
-
-      hred_r. remove_tau. unhide. remove_tau.
-      des_ifs_safe. hred_r.
-      hred_l. iApply isim_choose_src. iExists _.
-      iApply isim_ret.
-      iFrame. iSplit; ss.
-      iPureIntro. f_equal.
-      autounfold with ptrArith in *. des_ifs_safe.
-      f_equal. unfold Vnullptr in *. unfold Ptrofs.xor.
-      des_ifs_safe.
-      autorewrite with ptrArith; auto with ptrArith.
-      unfold Int64.zero. autorewrite with ptrArith.
-      2:{ set Int64.max_unsigned. vm_compute in z. nia. }
-      rewrite Z.lxor_0_r. et.
-  Qed. *)
-  Admitted. *)
 
   End SIMFUNS.
 
-  Opaque Sk.canon.
 
-  Theorem correct : refines2 [xorlist0.xor] [xorlist1.xor GlobalStb].
+Require Import ClightDmMem01Proof.
+
+  Theorem correct : refines2 [xorlist0.xor; ClightDmMem0.Mem] [xorlist1.xor GlobalStb; ClightDmMem1.Mem].
   Proof.
-    eapply adequacy_local2. econs; ss.
-    i. econstructor 1 with (wf := wf) (le := top2); et; ss; cycle 1.
+    eapply adequacy_local_strong_l. econs; cycle 1.
+    { econs; ss. econs; ss. }
+    i. econs; ss; cycle 1.
+    { econs; ss. apply correct_mod; et. }
+    econstructor 1 with (wf := wf) (le := top2); et; ss; cycle 1.
     { eexists. econs. apply to_semantic. iIntros. et. }
     (* each functions has simulation relation *)
     econs; cycle 1.
@@ -1445,12 +1303,11 @@ Section PROOF.
     econs; cycle 1.
     econs; cycle 1.
     econs; et.
-    all: rewrite f_bind_ret_r; unfold get_ce; replace (map _ _) with ce by et.
-    - apply sim_search; et.
-    - apply sim_delete; et.
-    - apply sim_add; et.
-    - apply sim_decrypt; et.
-    - apply sim_encrypt; et.
+    all: des_ifs; inv SKINCL; inv H6; ss.
+    - apply sim_delete_tl; et.
+    - apply sim_delete_hd; et.
+    - apply sim_add_tl; et.
+    - apply sim_add_hd; et.
     Unshelve. exact tt.
   Qed.
 
